Cpc/Logos.lean
@@ -8376,6 +8376,9 @@ def __eo_is_closed_rec : Term -> Term -> Term
   | (Term.Apply (Term.Apply (Term.UOp UserOp.forall) vs) x), env => (__eo_is_closed_rec x (__eo_list_concat Term.__eo_List_cons vs env))
   | (Term.Apply (Term.Apply (Term.UOp UserOp.exists) vs) x), env => (__eo_is_closed_rec x (__eo_list_concat Term.__eo_List_cons vs env))
   | (Term.Apply f x), env => (__eo_and (__eo_is_closed_rec f env) (__eo_is_closed_rec x env))
+  | (Term.UOp1 _ x), env => (__eo_is_closed_rec x env)
+  | (Term.UOp2 _ x y), env => (__eo_and (__eo_is_closed_rec x env) (__eo_is_closed_rec y env))
+  | (Term.UOp3 _ x y z), env => (__eo_and (__eo_and (__eo_is_closed_rec x env) (__eo_is_closed_rec y env)) (__eo_is_closed_rec z env))
   | x, env => (Term.Boolean true)
 
 
